aneris/examples/snapshot_isolation/examples/only_reads/only_reads_proof.v
@@ -62,15 +62,16 @@ Context `{!anerisG Mdl Σ, !SI_resources Mdl Σ, !SI_client_toolbox, !KVSG Σ}.
   {{{ inv client_inv_name client_inv
     ∗ client_1_addr ⤳ (∅, ∅)
     ∗ unallocated {[client_1_addr]}
+    ∗ KVS_ClientCanConnect (SocketAddressInet ip port)
     ∗ free_ports ip {[port]}
     ∗ KVS_address ⤇ KVS_si }}}
     transaction1_client $client_1_addr $KVS_address @[ip]
   {{{ v, RET v; True }}}.
   Proof.
-    iIntros (Hip Hports Φ) "(#Hinv & Hmsghis & Hunalloc
+    iIntros (Hip Hports Φ) "(#Hinv & Hmsghis & Hunalloc & Hcc
     & Hports & Hprot) HΦ".
     rewrite /transaction1_client. wp_pures. rewrite Hip Hports.
-    wp_apply (SI_init_client_proxy_spec with "[$Hunalloc $Hprot $Hmsghis $Hports]").
+    wp_apply (SI_init_client_proxy_spec with "[$Hunalloc $Hprot $Hmsghis $Hports $Hcc]").
     iIntros (rpc) "(Hcstate & #HiC)".
     wp_pures. rewrite /transaction1. wp_pures.
     wp_apply (SI_start_spec $! rpc client_1_addr (⊤ ∖ ↑client_inv_name)); try solve_ndisj.
@@ -116,15 +117,16 @@ Context `{!anerisG Mdl Σ, !SI_resources Mdl Σ, !SI_client_toolbox, !KVSG Σ}.
     {{{ inv client_inv_name client_inv
       ∗ client_2_addr ⤳ (∅, ∅)
       ∗ unallocated {[client_2_addr]}
+      ∗ KVS_ClientCanConnect (SocketAddressInet ip port)
       ∗ free_ports ip {[port]}
       ∗ KVS_address ⤇ KVS_si }}}
       transaction2_client $client_2_addr $KVS_address @[ip]
     {{{ v, RET v; True }}}.
   Proof.
-    iIntros (Hip Hports Φ) "(#Hinv & Hmsghis & Hunalloc
+    iIntros (Hip Hports Φ) "(#Hinv & Hmsghis & Hunalloc & Hcc
     & Hports & Hprot) HΦ".
     rewrite /transaction2_client. wp_pures. rewrite Hip Hports.
-    wp_apply (SI_init_client_proxy_spec with "[$Hunalloc $Hprot $Hmsghis $Hports]").
+    wp_apply (SI_init_client_proxy_spec with "[$Hunalloc $Hprot $Hmsghis $Hports $Hcc]").
     iIntros (rpc) "(Hcstate & #HiC)". wp_pures.
     rewrite /transaction2. wp_pures.
     wp_apply (SI_start_spec $! rpc client_2_addr (⊤ ∖ ↑client_inv_name)); try solve_ndisj.
@@ -186,7 +188,9 @@ Context `{!anerisG Mdl Σ, !SI_init, !KVSG Σ}.
       example_runner @["system"]
     {{{ v, RET v; True }}}.
   Proof.
-    iMod SI_init_module as (SI_res SI_client_toolbox) "(HKVSres & HVKSinit)".
+    iMod (SI_init_module _ {[client_1_addr; client_2_addr]}) as
+      (SI_res SI_client_toolbox)
+                             "(HKVSres & HVKSinit & Hcc)".
     iMod (inv_alloc client_inv_name ⊤ (client_inv) with "[HKVSres]") as "#Hinv".
     { iNext. iExists [].
     iDestruct (big_sepS_delete _ _ "x" with "HKVSres") as "(Hx & HKVSres)";
@@ -200,15 +204,21 @@ Context `{!anerisG Mdl Σ, !SI_init, !KVSG Σ}.
     iIntros "#HKVS_si".
     wp_apply (aneris_wp_start {[80%positive]}).
     iFrame.
+    iDestruct (big_sepS_delete _  _ client_1_addr with "Hcc")
+      as "(Hcc1 & Hcc)";
+    first set_solver.
+    iDestruct (big_sepS_delete _  _ client_2_addr with "Hcc")
+      as "(Hcc2 & _)";
+    first set_solver.
     iSplitR "Hsrvhist HVKSinit".
     - iModIntro. wp_pures.
       wp_apply (aneris_wp_start {[80%positive : port]}).
       iFrame.
-      iSplitR "Hcli1hist Hcli1unalloc".
+      iSplitR "Hcli1hist Hcli1unalloc Hcc1".
       + iModIntro. wp_pures.
         wp_apply (aneris_wp_start {[80%positive : port]}).
         iFrame.
-        iSplitR "Hcli2hist Hcli2unalloc".
+        iSplitR "Hcli2hist Hcli2unalloc Hcc2".
         * by iApply "HΦ".
         * iIntros "!> Hports". wp_apply (client_2_spec with "[$]"); try done.
       + iIntros "!> Hports". wp_apply (client_1_spec with "[$]"); try done.
